libs/ffi/FFICallbacks.fst
@@ -17,14 +17,14 @@ assume val ocaml_recv_tcp: cb_state -> string -> Tot int
 assume val ocaml_ticket_cb: cb_state -> cb_fun_ptr -> string -> bytes -> bytes -> EXT unit
 
 // Certificate callbacks
-assume val ocaml_cert_select_cb: cb_state -> cb_fun_ptr -> pv:int -> sni:string * alpn:bytes -> sigalgs:bytes -> EXT (option (cert_ptr * sigalg))
+assume val ocaml_cert_select_cb: cb_state -> cb_fun_ptr -> pv:int -> (*sni:*)string * (*alpn:*)bytes -> sigalgs:bytes -> EXT (option (cert_ptr * sigalg))
 assume val ocaml_cert_format_cb: cb_state -> cb_fun_ptr -> cert_ptr -> EXT bytes
 assume val ocaml_cert_sign_cb: cb_state -> cb_fun_ptr -> cert_ptr -> sigalg -> tbs:bytes -> EXT (option bytes)
-assume val ocaml_cert_verify_cb: cb_state -> cb_fun_ptr -> bytes -> sigalg -> tbs:bytes * sigv:bytes -> EXT bool
+assume val ocaml_cert_verify_cb: cb_state -> cb_fun_ptr -> bytes -> sigalg -> (*tbs:*)bytes * (*sigv:*)bytes -> EXT bool
 
 (* under the covers, recv invokes String.Substring, which may throw an exception
    due to invalid parameters.  But the recv codepath never does that.  However,
    The F* compiler does not know that.  So implement FFI recv in ML to avoid
    exposing the String.Substring call to effects checking.  Same as
    Platform.Tcp.recv *)
-assume val recvcb: callbacks -> max:nat -> EXT (result:bool * b:string {length (bytes_of_string b) <= max})
+assume val recvcb: callbacks -> max:nat -> EXT ((*result:*)bool * b:string {length (bytes_of_string b) <= max})
