src/tls/Token.UF1CMA.fst
@@ -105,7 +105,7 @@ let footprint (#ip:ipkg) (#i:ip.Pkg.t {ip.Pkg.registered i}) (k:key ip i):
 val create:
   ip:ipkg -> ha_of_i: (ip.Pkg.t -> ha) -> good_of_i: (ip.Pkg.t -> bool) ->
   i:ip.Pkg.t {ip.Pkg.registered i} ->
-  u:info {u.alg = ha_of_i i /\ u.good == good_of_i i} -> ST (k:key ip i)
+  u:info {u.alg = ha_of_i i /\ u.good == good_of_i i} -> ST (key ip i)
   (requires fun _ -> model)
   (ensures fun h0 k h1 ->
     modifies Set.empty h0 h1 /\
@@ -145,7 +145,7 @@ val coerce:
   ip: ipkg -> ha_of_i: (ip.Pkg.t -> ha) -> good_of_i: (ip.Pkg.t -> bool) ->
   i: ip.Pkg.t {ip.Pkg.registered i /\ ~(safe i)} ->
   u: info {u.alg = ha_of_i i /\ u.good == good_of_i i} ->
-  kv: lbytes32 (keylen u) -> ST (k:key ip i)
+  kv: lbytes32 (keylen u) -> ST (key ip i)
   (requires fun _ -> True)
   (ensures fun h0 k h1 ->
     modifies_none h0 h1 /\
